__1. Reverse the direction of the moving shell and re-derive the relationships of $\Delta t_{eng}$, $\Delta t_e$ and $\Delta t_{obs}$.__

__Proof__:

Just like the original derivation, but set the ejecta to move towards the shell.

Assuming at time moment $t_{eng1}$, a light singal began to emit from central engine (CE) and arrived at the ejecta point A at $t_{e1}$. Afterthat, it was absorbed and re-emitted towards the observer at an angle $\theta$ with respect to the radial direction and was detected at $t_{obs1}$.

After a time interval $\Delta t_{eng}$, _i.e._ at time $t_{eng2}=t_{eng1}+\Delta t_{eng}$, emission from the CE has been shutdown and the final emission photon left the ejecta point at $t_{e2}=t_{e1}+\Delta t_{e}$ and was finally observed at $t_{obs2}=t_{obs1}+\Delta t_{obs}$ by the observor. Set the ejecta co-moving frame velocity to be $v$, then the travel length difference between CE and the moving ejecta from the beginning to ending of the emission would be:

$$
\Delta r = r_2-r_1 = c(t_{e2}-t_{eng2}) - c(t_{e1}-t_{eng1}) = -v \Delta t_e
$$

The difference is negative since the ejecta is moving towards center, thus we have:

$$
c\Delta t_e - c\Delta t_{eng} = -v \Delta t_e
$$

$$
\Delta t_{eng} = (1+\beta)\Delta t_e
$$

Similarly, the ejecta shrinks $v\Delta t_e \cos\theta$ at the line of sight during time period $\Delta t_e$, and the light travel difference is positive (latter goes further):

$$
\Delta l = l_2-l_1 = c(t_{obs2}-t_{e2}) - c(t_{obs1}-t_{e1}) = v\Delta t_e \cos\theta
$$

$$
c\Delta t_{obs} - c\Delta t_{e} = v \Delta t_e\cos\theta
$$

$$
\Delta t_{obs} = (1+\beta\cos\theta)\Delta t_{e}
$$

In conclusion, we have:

$$
\Delta t_{eng}:\Delta t_{e}:\Delta t_{obs} = (1+\beta):1:(1+\beta\cos\theta)
$$